Transform.v
@@ -13,7 +13,7 @@ Require Import LLIR.Verify.
 
 
 
-Definition rewrite_uses (i: inst) (f: reg -> reg): inst :=
+Definition rewrite_inst_uses (i: inst) (f: reg -> reg): inst :=
   match i with
   | LLLd addr dst next => LLLd (f addr) dst next
   | LLSt addr val next => LLSt (f addr) (f val) next
@@ -35,12 +35,35 @@ Definition rewrite_uses (i: inst) (f: reg -> reg): inst :=
   | LLBinop ty op lhs rhs dst next => LLBinop ty op (f lhs) (f rhs) dst next
   end.
 
-
-Theorem use_rewritten:
-  forall (i: inst) (src: reg) (f: reg -> reg),
-    Uses i src -> Uses (rewrite_uses i f) (f src).
+Theorem inst_use_rewritten:
+  forall (i: inst) (r: reg) (f: reg -> reg),
+    InstUses i r -> InstUses (rewrite_inst_uses i f) (f r).
 Proof.
   destruct i; intros src f Huse; simpl; inversion Huse; try rewrite H; auto.
   right. apply List.in_map_iff. exists src.
   split. reflexivity. apply H.
+Qed.
+
+Definition rewrite_phi_uses (p: phi) (f: reg -> reg): phi :=
+  match p with
+  | LLPhi ins dst => LLPhi (List.map (fun phi_in =>
+    match phi_in with
+    | (block, r) => (block, f r)
+    end) ins) dst
+  end.
+
+Theorem phi_use_rewritten:
+  forall (p: phi) (n: node) (r: reg) (f: reg -> reg),
+    PhiUses p n r -> PhiUses (rewrite_phi_uses p f) n (f r).
+Proof.
+  destruct p; intros n r f Huse; simpl.
+  unfold PhiUses in Huse.
+  apply Exists_exists in Huse.
+  destruct Huse as [[n' r'] [Hin [Hn Hr]]]. subst n' r'.
+  apply Exists_exists.
+  exists (n, f r).
+  split; auto.
+  apply in_map_iff.
+  exists (n, r).
+  auto.
 Qed.
